WIP

src/dup.v
@@ -2,9 +2,63 @@ Set Implicit Arguments.
 Set Asymmetric Patterns.
 
 Require Import List.
+Import ListNotations.
 
 Require Import comparable.
 Require Import sort.
+
+Section inductive_predicate_strictly_sorted.
+  (* Being strictly sorted can be defined in two equivalent ways:
+1. being sorted and having no duplicates; or
+2. every element in the list is strictly smaller than the next.
+   *)
+
+  Context {A: Type}.
+  Context {cmp: comparable A}.
+
+  Inductive is_strictly_sorted : list A -> Prop :=
+  | empty_strictly_sorted : is_strictly_sorted nil
+  | singleton_strictly_sorted (x : A) : is_strictly_sorted [x]
+  | tail_strictly_sorted (x y : A) (xs : list A):
+      (compare x y = Lt)
+      -> is_strictly_sorted (y :: xs)
+      -> is_strictly_sorted (x :: y :: xs).
+
+  Hint Constructors is_strictly_sorted : strictly_sorted.
+
+  Lemma is_strictly_sorted_tail: forall (ls : list A),
+      is_strictly_sorted ls -> is_strictly_sorted (tl ls).
+  Proof.
+    intro ls. intro H.
+    destruct H; auto with strictly_sorted.
+  Qed.
+End inductive_predicate_strictly_sorted.
+
+Section remove_duplicates_from_sorted.
+  Context {A: Type}.
+  Context {cmp: comparable A}.
+
+  (* The type of this function does not entirely specify the function: the
+     result may be a strictly sorted list, but there is nothing that says it is
+     the same as ls, but with duplicates removed. *)
+  Fixpoint remove_duplicates_from_sorted (ls : list A):
+      is_sorted ls -> {ls' : list A | is_strictly_sorted ls'}.
+    intro.
+    (* Probably need to do convoy trick here again. *)
+    refine (match ls with
+              | nil => (exist _ nil empty_strictly_sorted)
+              | (x0 :: xs')
+                => match xs' with
+                   | nil => (exist _ [x0] (singleton_strictly_sorted x0))
+                   | (x1 :: xs'') =>
+                     match compare x0 x1 with
+                     | Eq => remove_duplicates_from_sorted xs' (tail_of_is_sorted_is_sorted H)
+                     | _ => x0 :: (remove_duplicates_from_sorted xs' (tail_of_is_sorted_is_sorted H))
+                     end
+                   end
+            end).
+  Abort.
+End remove_duplicates_from_sorted.
 
 (* remove_duplicates_from_sorted removes duplicates from a sorted list *)
 Fixpoint remove_duplicates_from_sorted {A: Type} {cmp: comparable A} (xs: list A): list A :=
